src/3d/Binding.fsti
@@ -41,7 +41,7 @@ val bit_order_of_integral_typ (_:env) (_:typ) (_:range) : ML bitfield_bit_order
 val bind_decls (g:global_env) (p:list decl) : ML (list decl & global_env)
 //val add_field_error_code_decls (ge: env) : ML (list decl)
 
-val initial_global_env (_:unit) : ML global_env
+val initial_global_env (mname:string) : ML global_env
 // DOES NOT return exported output types/extern types/extern functions
 val get_exported_decls (ge:global_env) (mname:string) : ML (list ident' & list ident')  //exported, private
 val finish_module (ge:global_env) (mname:string)
